FOL part done

theories/Semantics/FOL/Syntax.v
@@ -1,9 +1,7 @@
 From stdpp Require Import prelude.
-From Coq Require Import Classical.
 
 From sets Require Import Ensemble Functions.
 
-From Semantics.Utils Require Import SetsExtras.
 
 Inductive Formula (V : Type) (A : Type -> Type) :=
 | Atomic (a : A V)
@@ -41,27 +39,6 @@ end.
 Definition statement A `{FreeVars A V} : Ensemble A :=
     fun phi => free_vars phi ≡ ∅.
 
-Definition vec_ct `(c : A) : vec A 0 -> A := const c.
-Definition vec_op1 `(f : A -> A) (a : vec A 1) : A :=
-    f (a !!! 0%fin).
-Definition vec_op2 `(f : A -> A -> A) (a : vec A 2) : A :=
-    f (a !!! 0%fin) (a !!! 1%fin).
-Definition vec_op3 `(f : A -> A -> A -> A) (a : vec A 3) : A :=
-    f (a !!! 0%fin) (a !!! 1%fin) (a !!! 2%fin).
-Definition vec_op4 `(f : A -> A -> A -> A -> A) (a : vec A 4) : A :=
-    f (a !!! 0%fin) (a !!! 1%fin) (a !!! 2%fin) (a !!! 3%fin).
-
-Definition vec_r0 `{A} (f : Prop) : vec A 0 -> Prop :=
-    const f.
-Definition vec_r1 `(f : A -> Prop) (a : vec A 1) : Prop :=
-    f (a !!! 0%fin).
-Definition vec_r2 `(f : A -> A -> Prop) (a : vec A 2) : Prop :=
-    f (a !!! 0%fin) (a !!! 1%fin).
-Definition vec_r3 `(f : A -> A -> A -> Prop) (a : vec A 3) : Prop :=
-    f (a !!! 0%fin) (a !!! 1%fin) (a !!! 2%fin).
-Definition vec_r4 `(f : A -> A -> A -> A -> Prop) (a : vec A 4) : Prop :=
-    f (a !!! 0%fin) (a !!! 1%fin) (a !!! 2%fin) (a !!! 3%fin).
-
 Record signature : Type := {
 symbol : Type;
 relation : Type;
@@ -72,291 +49,8 @@ r_arity : relation -> nat;
 Arguments s_arity {s} _: assert.
 Arguments r_arity {s} _: assert.
 
-Record structure (sigma : signature) : Type := {
-support : Type;
-op_interp (s : symbol sigma) : vec support (s_arity s) -> support;
-rel_interp (s : relation sigma) : vec support (r_arity s) -> Prop;
-}.
-
-Arguments support {sigma} s0 : assert.
-Arguments op_interp {sigma} s0 s _ : assert.
-Arguments rel_interp {sigma} s0 s _ : assert.
-
-Section sec_structure_examples.
-
-Inductive e1_symbols := Dot1 | Zero1 | One1 .
-Definition e1_s_arity (s : e1_symbols) : nat :=
-match s with
-| Dot1 => 2
-| _ => 0
-end.
-
-Definition e1_r_arity (s : False) : nat :=
-match s with
-end.
-
-Definition e1_signature : signature := {|
-symbol := e1_symbols;
-relation := False;
-s_arity := e1_s_arity;
-r_arity := e1_r_arity;
-|}.
-
-Definition e1_op_interp  (s : symbol e1_signature) : vec Z (s_arity s) -> Z :=
-match s as e return (vec Z (@s_arity e1_signature e) → Z)
-with
-| Dot1 => vec_op2 Z.add
-| Zero1 => vec_ct 2%Z
-| One1 => vec_ct 7%Z
-end.
-
-Definition e1_structure : structure e1_signature := {|
-support := Z;
-op_interp := e1_op_interp;
-rel_interp := fun s => match s with end
-|}.
-
-Inductive e2_relations := Le2.
-
-Definition e2_r_arity : e2_relations -> nat := const 2.
-
-Definition e2_signature : signature := {|
-symbol := False;
-relation := e2_relations;
-s_arity := fun s => match s with end;
-r_arity := e2_r_arity;
-|}.
-
-Definition e2_rel_interp (s : relation e2_signature) : vec nat (r_arity s) -> Prop :=
-match s as e return (vec nat (@r_arity e2_signature e) → Prop)
-with
-| Le2 => vec_r2 (fun x y => x > y)
-end.
-
-Definition e2_structure : structure e2_signature := {|
-support := nat;
-op_interp := fun (s : symbol e2_signature) => match s with end;
-rel_interp := e2_rel_interp;
-|}.
-
-Inductive e3_relation := I3 | A3 | B3.
-
-Definition e3_signature : signature := {|
-symbol := False;
-relation := e3_relation;
-s_arity := fun s => match s with end;
-r_arity := const 1;
-|}.
-
-Inductive eq_relation := EqS.
-
-Definition eq_signature : signature := {|
-symbol := False;
-relation := eq_relation;
-s_arity := fun s => match s with end;
-r_arity := const 2;
-|}.
-
-Inductive arith_symbol := SAdd | SMul | SS | S0.
-
-Inductive arith_relation := RLt.
-
-Definition arith_s_arity (s : arith_symbol) : nat :=
-match s with
-| SAdd => 2
-| SMul => 2
-| SS => 1
-| S0 => 0
-end.
-
-Definition arith_r_arity : arith_relation -> nat := const 2.
-
-Definition arith_signature : signature := {|
-symbol := arith_symbol;
-relation := arith_relation;
-s_arity := arith_s_arity;
-r_arity := arith_r_arity;
-|}.
-
-
-Definition nat_op_interp (s : symbol arith_signature) : vec nat (s_arity s) -> nat :=
-match s as e return (vec nat (@s_arity arith_signature e) → nat)
-with
-| SAdd => vec_op2 Nat.add
-| SMul => vec_op2 Nat.mul
-| SS => vec_op1 S
-| S0 => vec_ct 0
-end.
-
-Definition nat_rel_interp (s : relation arith_signature) : vec nat (r_arity s) -> Prop :=
-match s as e return (vec nat (@r_arity arith_signature e) → Prop)
-with
-| Rlt => vec_r2 (fun x y => x < y)
-end.
-
-Definition nat_structure : structure arith_signature := {|
-support := nat;
-op_interp := nat_op_interp;
-rel_interp := nat_rel_interp;
-|}.
-
-Definition arith_bool_op_interp (s : symbol arith_signature) : vec bool (s_arity s) -> bool :=
-match s as e return (vec bool (@s_arity arith_signature e) → bool)
-with
-| SAdd => vec_op2 andb
-| SMul => vec_op2 orb
-| SS => vec_op1 negb
-| S0 => vec_ct false
-end.
-
-Definition arith_bool_rel_interp (s : relation arith_signature) : vec bool (r_arity s) -> Prop :=
-match s as e return (vec bool (@r_arity arith_signature e) → Prop)
-with
-| Rlt => vec_r2 implb
-end.
-
-Definition arith_bool_structure : structure arith_signature := {|
-support := bool;
-op_interp := arith_bool_op_interp;
-rel_interp := arith_bool_rel_interp;
-|}.
-
-End sec_structure_examples.
-
-
-Class Satisfaction (sigma : signature) (V F : Type) :=
-    vsat_set : forall (M : structure sigma), F -> (V -> support M) -> Ensemble True.
-#[global] Hint Mode Satisfaction ! - ! : typeclass_instances.
-
-Section sec_satisfaction_defs.
-
-Context `{Satisfaction}.
-
-Definition vsat (M : structure sigma) (f : F) (v : V -> support M) : Prop :=
-    vsat_set M f v ≡ top True.
-
-Definition sat (M : structure sigma) (f : F) : Prop :=
-    forall (v : V -> support M), vsat M f v.
-
-Definition valid (f : F) : Prop :=
-    forall (M : structure sigma), sat M f.
-
-Definition satisfiable (f : F) : Prop :=
-    exists (M : structure sigma), sat M f.
-
-Definition unsatisfiable (f : F) : Prop := ~ satisfiable f.
-
-Definition sem_ded (f g : F) : Prop :=
-    forall (M : structure sigma), sat M f -> sat M g.
-
-Definition sat_set (M : structure sigma) (Gamma : Ensemble F) :=
-    forall (f : F), f ∈ Gamma -> sat M f.
-
-Definition satisfiable_set (Gamma : Ensemble F) :=
-    exists (M : structure sigma), sat_set M Gamma.
-
-Definition unsatisfiable_set (Gamma : Ensemble F) := ~ satisfiable_set Gamma.
-
-End sec_satisfaction_defs.
-
-Fixpoint f_sat {sigma} `{EqDecision V} {A} (a_sat : forall (M : structure sigma), (A V) -> (V -> support M) -> Ensemble True)
-    (M : structure sigma) (f : Formula V A) (v : V -> support M) :=
-match f with
-| Atomic a => a_sat M a v
-| Bot => ∅
-| Impl f g => complement (f_sat a_sat M f v) ∪ (f_sat a_sat M g v)
-| All x f => indexed_intersection (fun (a : support M) => f_sat a_sat M f (fn_update v x a))
-end.
-
-#[export] Instance formula_satisfaction `{EqDecision V} `{Satisfaction sigma V (A V)} :
-    Satisfaction sigma V (Formula V A) := f_sat vsat_set.
-
-Section vsat_props.
-
-Context {sigma : signature} `{EqDecision V} `{Satisfaction sigma V (A V)}  (M : structure sigma).
-
-Lemma vsat_atomic : forall (a : A V) (v : V -> support M),
-    vsat M (Atomic a) v <-> vsat M a v.
-Proof. done. Qed.
-
-Lemma vsat_bot : forall (v : V -> support M),
-    ~ vsat M (@Bot V A) v.
-Proof.
-    intros; unfold vsat, vsat_set; cbn.
-    by intro; apply top_not_bottom; symmetry.
-Qed.
-
-Lemma vsat_impl : forall (f g : Formula V A) (v : V -> support M),
-    vsat M (Impl f g) v <-> (vsat M f v -> vsat M g v).
-Proof.
-    intros; unfold vsat; cbn.
-    rewrite !top_char, elem_of_union, elem_of_complement.
-    split.
-    - by intros [] ?.
-    - intros Himpl.
-      destruct (classic (I ∈ vsat_set M f v)); [| by left].
-      by right; apply Himpl.
-Qed.
-
-Lemma vsat_all : forall (x : V) (f : Formula V A) (v : V -> support M),
-    vsat M (All x f) v <-> forall a, vsat M f (fn_update v x a).
-Proof.
-    intros; unfold vsat; cbn.
-    setoid_rewrite top_char.
-    by rewrite elem_of_indexed_intersection.
-Qed.
-
-Lemma vsat_top : forall (v : V -> support M),
-    vsat M (@f_top V A) v.
-Proof. by intros; apply vsat_impl. Qed.
-
-Lemma vsat_neg : forall (f : Formula V A) (v : V -> support M),
-    vsat M (f_neg f) v <-> ~ vsat M f v.
-Proof.
-    intros; unfold f_neg; rewrite vsat_impl; split.
-    - intros Hneg Hf.
-      by eapply vsat_bot, Hneg.
-    - by intros ? ?.
-Qed.
-
-Lemma vsat_and : forall (f g: Formula V A) (v : V -> support M),
-    vsat M (f_and f g) v <-> vsat M f v /\ vsat M g v.
-Proof.
-    intros; unfold f_and.
-    rewrite vsat_neg, vsat_impl, vsat_neg.
-    by tauto.
-Qed.
-
-Lemma vsat_or : forall (f g: Formula V A) (v : V -> support M),
-    vsat M (f_or f g) v <-> vsat M f v \/ vsat M g v.
-Proof.
-    intros; unfold f_or.
-    rewrite vsat_impl, vsat_neg.
-    by tauto.
-Qed.
-
-Lemma vsat_iff : forall (f g: Formula V A) (v : V -> support M),
-    vsat M (f_iff f g) v <-> (vsat M f v <-> vsat M g v).
-Proof.
-    intros; unfold f_iff.
-    rewrite vsat_and, !vsat_impl.
-    by tauto.
-Qed.
-
-Lemma vsat_ex : forall (x : V) (f : Formula V A) (v : V -> support M),
-    vsat M (f_ex x f) v <-> exists (a : support M), vsat M f (fn_update v x a).
-Proof.
-    intros; unfold f_ex.
-    rewrite vsat_neg, vsat_all.
-    setoid_rewrite vsat_neg.
-    split.
-    - by intro; apply not_all_not_ex.
-    - intros [z Hz] Hall.
-      by eapply Hall.
-Qed.
-
-End vsat_props.
-
+Class EnsuringInhabitation (sigma : signature) :=
+    ensures_inhabitation : {s : symbol sigma & s_arity s = 0}.
 
 Section sec_terms.
 
@@ -414,11 +108,20 @@ Arguments Var {V%type_scope} v : assert.
 Arguments App {V%type_scope} s t : assert.
 
 Definition vterm_vars {V} : VTerm V -> listset V :=
-    vterm_rect V (fun _ => listset V) (fun _ _ => list (listset V))
+    vterm_rect V (fun _ => listset V) (fun n _ => vec (listset V) n)
       (fun v => {[v]})
       (fun _ _ ls => ⋃ ls)
-      []
-      (fun _ _ vt _ vts =>  vt :: vts).
+      [#]
+      (fun _ _ vt _ vts =>  vt ::: vts).
+
+#[export] Instance vterm_free_vars V : FreeVars (VTerm V) V := vterm_vars.
+
+Lemma vterm_fv_var `(x : V) : free_vars (Var x) = {[x]}.
+Proof. done. Qed.
+
+Lemma vterm_fv_app {V} (s : symbol sigma) (ts : vec (VTerm V) (s_arity s)) :
+    free_vars (App s ts) = ⋃ vmap free_vars  ts.
+Proof. done. Qed.
 
 Definition Term : Type := VTerm False.
 
@@ -429,53 +132,71 @@ Definition term_to_vterm (V : Type) : Term -> VTerm V :=
       [#]
       (fun _ n v0 _ vl => v0 ::: vl).
 
-Lemma term_vars : forall (t : Term), vterm_vars t ≡ ∅.
+Lemma term_vars : forall (t : Term), free_vars t ≡ ∅.
 Proof.
     induction t using vterm_ind; cbn; [by inversion v |].
     apply empty_union_list, Forall_forall; intros.
     by rewrite elem_of_equiv_empty; intro.
 Qed.
 
-Definition vterm_eval (A : structure sigma) `(v : V -> support A) :
-    VTerm V -> support A :=
-    vterm_rect V (fun _ => support A) (fun n _ => vec (support A) n)
-      (fun x => v x)
-      (fun sigma _ va => op_interp A sigma va)
-      [#]
-      (fun _ n v0 _ vl => v0 ::: vl).
-
-Definition term_eval (A : structure sigma) : Term -> support A :=
-    vterm_eval A (fun (v : False) => match v with end).
-
 Inductive RelAtom (V : Type) :=
 | RApp (pi : relation sigma) (t : vec (VTerm V) (r_arity pi)).
 
+Definition rel_atom_vars {V} (ra : RelAtom V) : listset V :=
+    match ra with
+    | RApp _ pi ts => ⋃ map free_vars (vec_to_list ts)
+    end.
+
+#[export] Instance rel_atom_free_vars V : FreeVars (RelAtom V) V := rel_atom_vars.
+
 Inductive EqAtom (V : Type) :=
 | REq (l r : VTerm V).
+
+Definition eq_atom_vars {V} (ea : EqAtom V) : listset V :=
+    match ea with
+    | REq _ l r => free_vars l ∪ free_vars r
+    end.
+
+#[export] Instance eq_atom_free_vars V : FreeVars (EqAtom V) V := eq_atom_vars.
 
 Inductive RelEqAtom (V : Type) :=
 | ARel (ar : RelAtom V)
 | AEq (ae : EqAtom V).
 
+Definition rel_eq_atom_vars {V} (a : RelEqAtom V) : listset V :=
+    match a with
+    | ARel _ ar => free_vars ar
+    | AEq _ ae => free_vars ae
+    end.
+
+#[export] Instance rel_eq_atom_free_vars V : FreeVars (RelEqAtom V) V := rel_eq_atom_vars.
+
+Coercion ARel : RelAtom >-> RelEqAtom.
+Coercion AEq : EqAtom >-> RelEqAtom.
+
+Definition EqFormula (V : Type) := Formula V EqAtom.
+
 Definition RelFormula (V : Type) := Formula V RelAtom.
 
 Definition RelEqFormula (V : Type) := Formula V RelEqAtom.
 
-Definition eq_set_vsat {V} (A : structure sigma) (e : EqAtom V) `(v : V -> support A) :
-    Ensemble True :=
-match e with
-| REq _ l r => const (vterm_eval A v l = vterm_eval A v r)
+Fixpoint formula_eq_to_rel `(f : EqFormula V) : RelEqFormula V :=
+match f with
+| Atomic eq => Atomic (AEq _ eq)
+| Bot => Bot
+| Impl f g => Impl (formula_eq_to_rel f) (formula_eq_to_rel g)
+| All x f => All x (formula_eq_to_rel f)
 end.
 
-#[export] Instance eq_atom_satisfaction V : Satisfaction sigma V (EqAtom V) :=
-    eq_set_vsat.
-
-Definition rel_set_vsat {V} (A : structure sigma) (e : RelAtom V) `(v : V -> support A) : Ensemble True :=
-match e with
-| RApp _ pi ts => const (rel_interp A pi (vmap (vterm_eval A v) ts))
-end.
-
-#[export] Instance rel_atom_satisfaction V : Satisfaction sigma V (RelAtom V) :=
-    rel_set_vsat.
+Coercion formula_eq_to_rel : EqFormula >-> RelEqFormula.
 
 End sec_terms.
+
+Arguments Var {sigma V%type_scope} v : assert.
+Arguments App {sigma V%type_scope} s t : assert.
+
+Arguments RApp {sigma V%type_scope} pi t : assert.
+Arguments REq {sigma V%type_scope} l r : assert.
+
+Arguments ARel {sigma V%type_scope} ar : assert.
+Arguments AEq {sigma V%type_scope} ae : assert.
